<?xml version="1.0"?>
<rdf:RDF xmlns="http://www.semanticweb.org/lenovot480s/ontologies/2024/1/19/untitled-ontology-20/"
     xml:base="http://www.semanticweb.org/lenovot480s/ontologies/2024/1/19/untitled-ontology-20/"
     xmlns:owl="http://www.w3.org/2002/07/owl#"
     xmlns:rdf="http://www.w3.org/1999/02/22-rdf-syntax-ns#"
     xmlns:xml="http://www.w3.org/XML/1998/namespace"
     xmlns:xsd="http://www.w3.org/2001/XMLSchema#"
     xmlns:rdfs="http://www.w3.org/2000/01/rdf-schema#">
    <owl:Ontology rdf:about="http://www.semanticweb.org/lenovot480s/ontologies/2024/1/19/untitled-ontology-20"/>
    


    <!-- 
    ///////////////////////////////////////////////////////////////////////////////////////
    //
    // Object Properties
    //
    ///////////////////////////////////////////////////////////////////////////////////////
     -->

    


    <!-- http://www.semanticweb.org/lenovot480s/ontologies/2024/1/19/untitled-ontology-20#OWLObjectProperty_415ac432_6d04_4977_a546_4819b459d1f0 -->

    <owl:ObjectProperty rdf:about="http://www.semanticweb.org/lenovot480s/ontologies/2024/1/19/untitled-ontology-20#OWLObjectProperty_415ac432_6d04_4977_a546_4819b459d1f0">
        <rdfs:label xml:lang="en">DatasetModality</rdfs:label>
    </owl:ObjectProperty>
    


    <!-- 
    ///////////////////////////////////////////////////////////////////////////////////////
    //
    // Classes
    //
    ///////////////////////////////////////////////////////////////////////////////////////
     -->

    


    <!-- http://www.semanticweb.org/lenovot480s/ontologies/2024/1/19/untitled-ontology-20#OWLClass_03548e07_4985_4355_bf15_c3d113f33436 -->

    <owl:Class rdf:about="http://www.semanticweb.org/lenovot480s/ontologies/2024/1/19/untitled-ontology-20#OWLClass_03548e07_4985_4355_bf15_c3d113f33436">
        <rdfs:subClassOf rdf:resource="http://www.semanticweb.org/lenovot480s/ontologies/2024/1/19/untitled-ontology-20#OWLClass_f2a74229_b0e1_41b7_b9b9_feec1458e800"/>
        <rdfs:comment>A strategy that selects instances based on Gaussian Mixture Models. Value: Number of components</rdfs:comment>
        <rdfs:label xml:lang="en">GaussianMixtureModelSampling</rdfs:label>
    </owl:Class>
    


    <!-- http://www.semanticweb.org/lenovot480s/ontologies/2024/1/19/untitled-ontology-20#OWLClass_064fc8a7_0bbd_4c11_b087_61c2ce01b8bb -->

    <owl:Class rdf:about="http://www.semanticweb.org/lenovot480s/ontologies/2024/1/19/untitled-ontology-20#OWLClass_064fc8a7_0bbd_4c11_b087_61c2ce01b8bb">
        <rdfs:subClassOf rdf:resource="http://www.semanticweb.org/lenovot480s/ontologies/2024/1/19/untitled-ontology-20#OWLClass_fef00ae7_b551_4050_80d4_d530b152590f"/>
        <rdfs:comment>Active learning framework tailored to specific applications.Properties:- Application domain. Values:- Healthcare, - Finance, - E-commerce</rdfs:comment>
        <rdfs:label xml:lang="en">ApplicationSpecificFramework</rdfs:label>
    </owl:Class>
    


    <!-- http://www.semanticweb.org/lenovot480s/ontologies/2024/1/19/untitled-ontology-20#OWLClass_098e6aad_354a_4eb4_b318_aff91ddfa631 -->

    <owl:Class rdf:about="http://www.semanticweb.org/lenovot480s/ontologies/2024/1/19/untitled-ontology-20#OWLClass_098e6aad_354a_4eb4_b318_aff91ddfa631">
        <rdfs:subClassOf rdf:resource="http://www.semanticweb.org/lenovot480s/ontologies/2024/1/19/untitled-ontology-20#OWLClass_ddcafd3a_7b94_404c_9c2b_c92ebf4f89e0"/>
        <rdfs:comment xml:lang="en">A strategy that combines query synthesis and traditional active learning methods. Value: Synthesis method (e.g., membership querying)</rdfs:comment>
        <rdfs:label xml:lang="en">QuerySynthesisHybrid</rdfs:label>
    </owl:Class>
    


    <!-- http://www.semanticweb.org/lenovot480s/ontologies/2024/1/19/untitled-ontology-20#OWLClass_0b89c530_f673_48f4_92d5_9cfbedee3776 -->

    <owl:Class rdf:about="http://www.semanticweb.org/lenovot480s/ontologies/2024/1/19/untitled-ontology-20#OWLClass_0b89c530_f673_48f4_92d5_9cfbedee3776">
        <rdfs:subClassOf rdf:resource="http://www.semanticweb.org/lenovot480s/ontologies/2024/1/19/untitled-ontology-20#OWLClass_da97fd0b_a17c_4ecb_be57_d12afa99ff07"/>
        <rdfs:comment>A strategy that selects the top instances with the highest margin ranks. Value:Number of top instances to select</rdfs:comment>
        <rdfs:label xml:lang="en">TopMarginRankingSampling</rdfs:label>
    </owl:Class>
    


    <!-- http://www.semanticweb.org/lenovot480s/ontologies/2024/1/19/untitled-ontology-20#OWLClass_0dbc8814_f314_4e28_8f20_4785023e09cb -->

    <owl:Class rdf:about="http://www.semanticweb.org/lenovot480s/ontologies/2024/1/19/untitled-ontology-20#OWLClass_0dbc8814_f314_4e28_8f20_4785023e09cb">
        <rdfs:subClassOf rdf:resource="http://www.semanticweb.org/lenovot480s/ontologies/2024/1/19/untitled-ontology-20#OWLClass_2d55bf6b_29fe_467e_8a00_6d4bab026699"/>
        <rdfs:comment>A strategy that selects instances with a balanced margin distribution.</rdfs:comment>
        <rdfs:label xml:lang="en">BalancedMarginSampling</rdfs:label>
    </owl:Class>
    


    <!-- http://www.semanticweb.org/lenovot480s/ontologies/2024/1/19/untitled-ontology-20#OWLClass_0deb7bbc_7452_4fc3_b65c_f57dbd3c2935 -->

    <owl:Class rdf:about="http://www.semanticweb.org/lenovot480s/ontologies/2024/1/19/untitled-ontology-20#OWLClass_0deb7bbc_7452_4fc3_b65c_f57dbd3c2935">
        <rdfs:subClassOf rdf:resource="http://www.semanticweb.org/lenovot480s/ontologies/2024/1/19/untitled-ontology-20#OWLClass_c13d0274_448e_45df_a089_4f811c399630"/>
        <rdfs:comment xml:lang="en">A strategy that selects instances based on cluster centroids. Value: Number of centroids, clustering algorithm</rdfs:comment>
        <rdfs:label xml:lang="en">ClusterCentroidSampling</rdfs:label>
    </owl:Class>
    


    <!-- http://www.semanticweb.org/lenovot480s/ontologies/2024/1/19/untitled-ontology-20#OWLClass_100f945c_10e2_4957_a71e_6d8ed203ee7f -->

    <owl:Class rdf:about="http://www.semanticweb.org/lenovot480s/ontologies/2024/1/19/untitled-ontology-20#OWLClass_100f945c_10e2_4957_a71e_6d8ed203ee7f">
        <rdfs:subClassOf rdf:resource="http://www.semanticweb.org/lenovot480s/ontologies/2024/1/19/untitled-ontology-20#OWLClass_2d55bf6b_29fe_467e_8a00_6d4bab026699"/>
        <rdfs:comment>A strategy that handles margin uncertainty in multi-class classification.</rdfs:comment>
        <rdfs:label xml:lang="en">MultiClassMarginSampling</rdfs:label>
    </owl:Class>
    


    <!-- http://www.semanticweb.org/lenovot480s/ontologies/2024/1/19/untitled-ontology-20#OWLClass_176d801d_88c5_475f_8446_ebf877b6c384 -->

    <owl:Class rdf:about="http://www.semanticweb.org/lenovot480s/ontologies/2024/1/19/untitled-ontology-20#OWLClass_176d801d_88c5_475f_8446_ebf877b6c384">
        <rdfs:subClassOf rdf:resource="http://www.semanticweb.org/lenovot480s/ontologies/2024/1/19/untitled-ontology-20#OWLClass_ddcafd3a_7b94_404c_9c2b_c92ebf4f89e0"/>
        <rdfs:comment xml:lang="en">A strategy that combines model-based and query-based active learning.</rdfs:comment>
        <rdfs:label xml:lang="en">ModelBasedActiveHybrid</rdfs:label>
    </owl:Class>
    


    <!-- http://www.semanticweb.org/lenovot480s/ontologies/2024/1/19/untitled-ontology-20#OWLClass_17fadee5_89bf_42f0_bd3e_265ddcfcb4af -->

    <owl:Class rdf:about="http://www.semanticweb.org/lenovot480s/ontologies/2024/1/19/untitled-ontology-20#OWLClass_17fadee5_89bf_42f0_bd3e_265ddcfcb4af">
        <rdfs:subClassOf rdf:resource="http://www.semanticweb.org/lenovot480s/ontologies/2024/1/19/untitled-ontology-20#OWLClass_c8b11866_3183_47ae_be50_a8e1a8186d37"/>
        <rdfs:comment>A strategy that selects instances with high entropy.</rdfs:comment>
        <rdfs:label xml:lang="en">HighEntropySampling</rdfs:label>
    </owl:Class>
    


    <!-- http://www.semanticweb.org/lenovot480s/ontologies/2024/1/19/untitled-ontology-20#OWLClass_187efe7f_96a3_44e2_aba1_bc3572664fb9 -->

    <owl:Class rdf:about="http://www.semanticweb.org/lenovot480s/ontologies/2024/1/19/untitled-ontology-20#OWLClass_187efe7f_96a3_44e2_aba1_bc3572664fb9">
        <rdfs:subClassOf rdf:resource="http://www.semanticweb.org/lenovot480s/ontologies/2024/1/19/untitled-ontology-20#OWLClass_c13d0274_448e_45df_a089_4f811c399630"/>
        <rdfs:comment xml:lang="en">A strategy that selects representative instances based on data density. Value: Density threshold, distance metric</rdfs:comment>
        <rdfs:label xml:lang="en">DensityBasedSampling</rdfs:label>
    </owl:Class>
    


    <!-- http://www.semanticweb.org/lenovot480s/ontologies/2024/1/19/untitled-ontology-20#OWLClass_19084a6d_45d5_4ca2_b0e5_1f26c52bcd2f -->

    <owl:Class rdf:about="http://www.semanticweb.org/lenovot480s/ontologies/2024/1/19/untitled-ontology-20#OWLClass_19084a6d_45d5_4ca2_b0e5_1f26c52bcd2f">
        <rdfs:subClassOf rdf:resource="http://www.semanticweb.org/lenovot480s/ontologies/2024/1/19/untitled-ontology-20#OWLClass_b476dd4b_0380_4dca_9da6_1bd7e8cd574f"/>
        <rdfs:comment>A strategy that selects instances based on variation ratio uncertainty.</rdfs:comment>
        <rdfs:label xml:lang="en">VariationRatioSampling</rdfs:label>
    </owl:Class>
    


    <!-- http://www.semanticweb.org/lenovot480s/ontologies/2024/1/19/untitled-ontology-20#OWLClass_1bda89b6_0141_4277_a609_a4c53452347d -->

    <owl:Class rdf:about="http://www.semanticweb.org/lenovot480s/ontologies/2024/1/19/untitled-ontology-20#OWLClass_1bda89b6_0141_4277_a609_a4c53452347d">
        <rdfs:subClassOf rdf:resource="http://www.semanticweb.org/lenovot480s/ontologies/2024/1/19/untitled-ontology-20#OWLClass_3b0030cc_7a96_45fa_8363_c8c60ab1a0ea"/>
        <rdfs:comment>Active learning scenario in a real-world application setting.Properties:- Application domain.Values:- Healthcare, - Finance, - E-commerce</rdfs:comment>
        <rdfs:label xml:lang="en">RealWorldScenario</rdfs:label>
    </owl:Class>
    


    <!-- http://www.semanticweb.org/lenovot480s/ontologies/2024/1/19/untitled-ontology-20#OWLClass_1d814d5b_e4fa_40db_bf4b_3d43ee31a2d7 -->

    <owl:Class rdf:about="http://www.semanticweb.org/lenovot480s/ontologies/2024/1/19/untitled-ontology-20#OWLClass_1d814d5b_e4fa_40db_bf4b_3d43ee31a2d7">
        <rdfs:subClassOf rdf:resource="http://www.semanticweb.org/lenovot480s/ontologies/2024/1/19/untitled-ontology-20#OWLClass_3e57c330_a8cc_48c0_afa0_daa39ae53ad8"/>
        <rdfs:label xml:lang="en">ActiveLearningDataset_V.1</rdfs:label>
    </owl:Class>
    


    <!-- http://www.semanticweb.org/lenovot480s/ontologies/2024/1/19/untitled-ontology-20#OWLClass_1fa5a787_09af_4cab_afd4_0e511f60e914 -->

    <owl:Class rdf:about="http://www.semanticweb.org/lenovot480s/ontologies/2024/1/19/untitled-ontology-20#OWLClass_1fa5a787_09af_4cab_afd4_0e511f60e914">
        <rdfs:subClassOf rdf:resource="http://www.semanticweb.org/lenovot480s/ontologies/2024/1/19/untitled-ontology-20#OWLClass_5949f4eb_04af_4e5f_a45b_67e5c4d21427"/>
        <rdfs:comment xml:lang="en">Combines predictions from multiple models.Properties:- Ensemble method. Values:- Voting, - Averaging, - Stacking</rdfs:comment>
        <rdfs:label xml:lang="en">EnsembleLearning</rdfs:label>
    </owl:Class>
    


    <!-- http://www.semanticweb.org/lenovot480s/ontologies/2024/1/19/untitled-ontology-20#OWLClass_294c43b6_7635_4a5d_8de1_c1aab60485e7 -->

    <owl:Class rdf:about="http://www.semanticweb.org/lenovot480s/ontologies/2024/1/19/untitled-ontology-20#OWLClass_294c43b6_7635_4a5d_8de1_c1aab60485e7">
        <rdfs:subClassOf rdf:resource="http://www.semanticweb.org/lenovot480s/ontologies/2024/1/19/untitled-ontology-20#OWLClass_5949f4eb_04af_4e5f_a45b_67e5c4d21427"/>
        <rdfs:comment>Updates the model incrementally as new data arrives.Properties: Learning rate. Values:	- Low, - Medium, - High</rdfs:comment>
        <rdfs:label xml:lang="en">OnlineLearning</rdfs:label>
    </owl:Class>
    


    <!-- http://www.semanticweb.org/lenovot480s/ontologies/2024/1/19/untitled-ontology-20#OWLClass_2d55bf6b_29fe_467e_8a00_6d4bab026699 -->

    <owl:Class rdf:about="http://www.semanticweb.org/lenovot480s/ontologies/2024/1/19/untitled-ontology-20#OWLClass_2d55bf6b_29fe_467e_8a00_6d4bab026699">
        <rdfs:subClassOf rdf:resource="http://www.semanticweb.org/lenovot480s/ontologies/2024/1/19/untitled-ontology-20#OWLClass_9f328153_8e29_4394_857a_48f04d38d710"/>
        <rdfs:comment>A strategy that selects instances based on margin uncertainty.</rdfs:comment>
        <rdfs:label xml:lang="en">MarginBasedInstanceSelection</rdfs:label>
    </owl:Class>
    


    <!-- http://www.semanticweb.org/lenovot480s/ontologies/2024/1/19/untitled-ontology-20#OWLClass_2eabbe26_6569_4248_a4ec_6899d5cfe478 -->

    <owl:Class rdf:about="http://www.semanticweb.org/lenovot480s/ontologies/2024/1/19/untitled-ontology-20#OWLClass_2eabbe26_6569_4248_a4ec_6899d5cfe478">
        <rdfs:subClassOf rdf:resource="http://www.semanticweb.org/lenovot480s/ontologies/2024/1/19/untitled-ontology-20#OWLClass_da97fd0b_a17c_4ecb_be57_d12afa99ff07"/>
        <rdfs:comment>A strategy that selects the bottom instances with the lowest margin ranks. Value: Number of bottom instances to select</rdfs:comment>
        <rdfs:label xml:lang="en">BottomMarginRankingSampling</rdfs:label>
    </owl:Class>
    


    <!-- http://www.semanticweb.org/lenovot480s/ontologies/2024/1/19/untitled-ontology-20#OWLClass_3082e515_0beb_4f06_86a1_77b804a503e4 -->

    <owl:Class rdf:about="http://www.semanticweb.org/lenovot480s/ontologies/2024/1/19/untitled-ontology-20#OWLClass_3082e515_0beb_4f06_86a1_77b804a503e4">
        <rdfs:subClassOf rdf:resource="http://www.semanticweb.org/lenovot480s/ontologies/2024/1/19/untitled-ontology-20#OWLClass_3b0030cc_7a96_45fa_8363_c8c60ab1a0ea"/>
        <rdfs:comment>Active learning scenario in a simulated environment.Propertes:- Simulation type. Values:- Synthetic data, - Generated scenarios</rdfs:comment>
        <rdfs:label xml:lang="en">SimulationScenario</rdfs:label>
    </owl:Class>
    


    <!-- http://www.semanticweb.org/lenovot480s/ontologies/2024/1/19/untitled-ontology-20#OWLClass_34ff58de_062c_4e73_8bf7_3299f7ec9b94 -->

    <owl:Class rdf:about="http://www.semanticweb.org/lenovot480s/ontologies/2024/1/19/untitled-ontology-20#OWLClass_34ff58de_062c_4e73_8bf7_3299f7ec9b94">
        <rdfs:subClassOf rdf:resource="http://www.semanticweb.org/lenovot480s/ontologies/2024/1/19/untitled-ontology-20#OWLClass_ddcafd3a_7b94_404c_9c2b_c92ebf4f89e0"/>
        <rdfs:comment>A strategy that combines instance selection and model update approaches. Value: Update frequency, selection criteria</rdfs:comment>
        <rdfs:label xml:lang="en">InstanceSelectionUpdateHybrid</rdfs:label>
    </owl:Class>
    


    <!-- http://www.semanticweb.org/lenovot480s/ontologies/2024/1/19/untitled-ontology-20#OWLClass_3928735c_5db3_4702_adbc_8b413817f54d -->

    <owl:Class rdf:about="http://www.semanticweb.org/lenovot480s/ontologies/2024/1/19/untitled-ontology-20#OWLClass_3928735c_5db3_4702_adbc_8b413817f54d">
        <rdfs:subClassOf rdf:resource="http://www.semanticweb.org/lenovot480s/ontologies/2024/1/19/untitled-ontology-20#OWLClass_99779c0f_ac3e_4a63_bafd_98dfcad0db0f"/>
        <rdfs:comment>A dataset with a fixed set of data instances available for labeling.Properties:Streaming method, Modality</rdfs:comment>
        <rdfs:label xml:lang="en">StreamBasedDataset</rdfs:label>
    </owl:Class>
    


    <!-- http://www.semanticweb.org/lenovot480s/ontologies/2024/1/19/untitled-ontology-20#OWLClass_3b0030cc_7a96_45fa_8363_c8c60ab1a0ea -->

    <owl:Class rdf:about="http://www.semanticweb.org/lenovot480s/ontologies/2024/1/19/untitled-ontology-20#OWLClass_3b0030cc_7a96_45fa_8363_c8c60ab1a0ea">
        <rdfs:subClassOf rdf:resource="http://www.semanticweb.org/lenovot480s/ontologies/2024/1/19/untitled-ontology-20#OWLClass_3e57c330_a8cc_48c0_afa0_daa39ae53ad8"/>
        <rdfs:label xml:lang="en">ActiveLearningScenario</rdfs:label>
    </owl:Class>
    


    <!-- http://www.semanticweb.org/lenovot480s/ontologies/2024/1/19/untitled-ontology-20#OWLClass_3d5b2170_8d30_4e65_8181_c62afa9d7761 -->

    <owl:Class rdf:about="http://www.semanticweb.org/lenovot480s/ontologies/2024/1/19/untitled-ontology-20#OWLClass_3d5b2170_8d30_4e65_8181_c62afa9d7761">
        <rdfs:subClassOf rdf:resource="http://www.semanticweb.org/lenovot480s/ontologies/2024/1/19/untitled-ontology-20#OWLClass_99779c0f_ac3e_4a63_bafd_98dfcad0db0f"/>
        <rdfs:comment xml:lang="en">A dataset with a fixed set of data instances available for labeling. Properties: Labeling method, Number of labeled instances, Modality</rdfs:comment>
        <rdfs:label xml:lang="en">PoolBasedDataset</rdfs:label>
    </owl:Class>
    


    <!-- http://www.semanticweb.org/lenovot480s/ontologies/2024/1/19/untitled-ontology-20#OWLClass_3e2f4525_72af_4015_86d2_72bc7df6240c -->

    <owl:Class rdf:about="http://www.semanticweb.org/lenovot480s/ontologies/2024/1/19/untitled-ontology-20#OWLClass_3e2f4525_72af_4015_86d2_72bc7df6240c">
        <rdfs:subClassOf rdf:resource="http://www.semanticweb.org/lenovot480s/ontologies/2024/1/19/untitled-ontology-20#OWLClass_2d55bf6b_29fe_467e_8a00_6d4bab026699"/>
        <rdfs:comment>A strategy that dynamically adjusts the margin threshold based on model performance.</rdfs:comment>
        <rdfs:label xml:lang="en">AdaptiveMarginSampling</rdfs:label>
    </owl:Class>
    


    <!-- http://www.semanticweb.org/lenovot480s/ontologies/2024/1/19/untitled-ontology-20#OWLClass_3e51d3f5_88cf_4c32_93e8_5b8d508e21fa -->

    <owl:Class rdf:about="http://www.semanticweb.org/lenovot480s/ontologies/2024/1/19/untitled-ontology-20#OWLClass_3e51d3f5_88cf_4c32_93e8_5b8d508e21fa">
        <rdfs:subClassOf rdf:resource="http://www.semanticweb.org/lenovot480s/ontologies/2024/1/19/untitled-ontology-20#OWLClass_f9d76460_e9ef_42a9_8aa2_94b6a52b0421"/>
        <rdfs:comment>Selects instances where model is expected to change most. Properties- Change measure. Values:- Information gain, - Model entropy change, - Gradient magnitude</rdfs:comment>
        <rdfs:label xml:lang="en">ExpectedModelChange</rdfs:label>
    </owl:Class>
    


    <!-- http://www.semanticweb.org/lenovot480s/ontologies/2024/1/19/untitled-ontology-20#OWLClass_3e57c330_a8cc_48c0_afa0_daa39ae53ad8 -->

    <owl:Class rdf:about="http://www.semanticweb.org/lenovot480s/ontologies/2024/1/19/untitled-ontology-20#OWLClass_3e57c330_a8cc_48c0_afa0_daa39ae53ad8">
        <rdfs:label xml:lang="en">ActiveLearning</rdfs:label>
    </owl:Class>
    


    <!-- http://www.semanticweb.org/lenovot480s/ontologies/2024/1/19/untitled-ontology-20#OWLClass_4067c745_c19d_4559_8372_f01dcd7cbb38 -->

    <owl:Class rdf:about="http://www.semanticweb.org/lenovot480s/ontologies/2024/1/19/untitled-ontology-20#OWLClass_4067c745_c19d_4559_8372_f01dcd7cbb38">
        <rdfs:subClassOf rdf:resource="http://www.semanticweb.org/lenovot480s/ontologies/2024/1/19/untitled-ontology-20#OWLClass_5949f4eb_04af_4e5f_a45b_67e5c4d21427"/>
        <rdfs:comment xml:lang="en">Co-trains multiple models on different views of the data. Properties:- Co-training method	Values:- Feature-based, - Instance-based, - Label-based</rdfs:comment>
        <rdfs:label xml:lang="en">CoTraining</rdfs:label>
    </owl:Class>
    


    <!-- http://www.semanticweb.org/lenovot480s/ontologies/2024/1/19/untitled-ontology-20#OWLClass_464e38f5_f411_42cc_8cb5_c97d0b1227eb -->

    <owl:Class rdf:about="http://www.semanticweb.org/lenovot480s/ontologies/2024/1/19/untitled-ontology-20#OWLClass_464e38f5_f411_42cc_8cb5_c97d0b1227eb">
        <rdfs:subClassOf rdf:resource="http://www.semanticweb.org/lenovot480s/ontologies/2024/1/19/untitled-ontology-20#OWLClass_fef00ae7_b551_4050_80d4_d530b152590f"/>
        <rdfs:comment>Active learning framework based on model update strategies.Properties:- Model update strategy. Values:- Retraining, - Online learning, - Transfer learning</rdfs:comment>
        <rdfs:label xml:lang="en">ModelBasedFramework</rdfs:label>
    </owl:Class>
    


    <!-- http://www.semanticweb.org/lenovot480s/ontologies/2024/1/19/untitled-ontology-20#OWLClass_47cb5da5_9dde_4805_ac2c_baee1fe0399c -->

    <owl:Class rdf:about="http://www.semanticweb.org/lenovot480s/ontologies/2024/1/19/untitled-ontology-20#OWLClass_47cb5da5_9dde_4805_ac2c_baee1fe0399c">
        <rdfs:subClassOf rdf:resource="http://www.semanticweb.org/lenovot480s/ontologies/2024/1/19/untitled-ontology-20#OWLClass_c13d0274_448e_45df_a089_4f811c399630"/>
        <rdfs:comment xml:lang="en">A strategy that selects representative instances from strata. Value: Strata definition, number of instances per strata</rdfs:comment>
        <rdfs:label xml:lang="en">StratifiedSampling</rdfs:label>
    </owl:Class>
    


    <!-- http://www.semanticweb.org/lenovot480s/ontologies/2024/1/19/untitled-ontology-20#OWLClass_48a72743_be39_4bbe_b5d2_9c40286910d1 -->

    <owl:Class rdf:about="http://www.semanticweb.org/lenovot480s/ontologies/2024/1/19/untitled-ontology-20#OWLClass_48a72743_be39_4bbe_b5d2_9c40286910d1">
        <rdfs:subClassOf rdf:resource="http://www.semanticweb.org/lenovot480s/ontologies/2024/1/19/untitled-ontology-20#OWLClass_3e57c330_a8cc_48c0_afa0_daa39ae53ad8"/>
        <rdfs:label xml:lang="en">QueryStrategy</rdfs:label>
    </owl:Class>
    


    <!-- http://www.semanticweb.org/lenovot480s/ontologies/2024/1/19/untitled-ontology-20#OWLClass_4b546552_bb11_4d6f_a2ea_7222b205898a -->

    <owl:Class rdf:about="http://www.semanticweb.org/lenovot480s/ontologies/2024/1/19/untitled-ontology-20#OWLClass_4b546552_bb11_4d6f_a2ea_7222b205898a">
        <rdfs:subClassOf rdf:resource="http://www.semanticweb.org/lenovot480s/ontologies/2024/1/19/untitled-ontology-20#OWLClass_2d55bf6b_29fe_467e_8a00_6d4bab026699"/>
        <rdfs:comment>A strategy that selects instances with a positive margin.</rdfs:comment>
        <rdfs:label xml:lang="en">PositiveMarginSampling</rdfs:label>
    </owl:Class>
    


    <!-- http://www.semanticweb.org/lenovot480s/ontologies/2024/1/19/untitled-ontology-20#OWLClass_5949f4eb_04af_4e5f_a45b_67e5c4d21427 -->

    <owl:Class rdf:about="http://www.semanticweb.org/lenovot480s/ontologies/2024/1/19/untitled-ontology-20#OWLClass_5949f4eb_04af_4e5f_a45b_67e5c4d21427">
        <rdfs:subClassOf rdf:resource="http://www.semanticweb.org/lenovot480s/ontologies/2024/1/19/untitled-ontology-20#OWLClass_3e57c330_a8cc_48c0_afa0_daa39ae53ad8"/>
        <rdfs:comment>different strategies for updating a machine learning model during the active learning process.</rdfs:comment>
        <rdfs:label xml:lang="en">ModelUpdateStrategy</rdfs:label>
    </owl:Class>
    


    <!-- http://www.semanticweb.org/lenovot480s/ontologies/2024/1/19/untitled-ontology-20#OWLClass_5b57ba8e_cb64_4902_9965_a7fb6602e95b -->

    <owl:Class rdf:about="http://www.semanticweb.org/lenovot480s/ontologies/2024/1/19/untitled-ontology-20#OWLClass_5b57ba8e_cb64_4902_9965_a7fb6602e95b">
        <rdfs:subClassOf rdf:resource="http://www.semanticweb.org/lenovot480s/ontologies/2024/1/19/untitled-ontology-20#OWLClass_f9d76460_e9ef_42a9_8aa2_94b6a52b0421"/>
        <rdfs:comment>Selects core set of representative instances.Properties:- Core set size. Values:- Small, - Medium, - Large</rdfs:comment>
        <rdfs:label xml:lang="en">CoreSetSelection</rdfs:label>
    </owl:Class>
    


    <!-- http://www.semanticweb.org/lenovot480s/ontologies/2024/1/19/untitled-ontology-20#OWLClass_5c32c93e_1b78_48d7_b141_331a571f6f47 -->

    <owl:Class rdf:about="http://www.semanticweb.org/lenovot480s/ontologies/2024/1/19/untitled-ontology-20#OWLClass_5c32c93e_1b78_48d7_b141_331a571f6f47">
        <rdfs:subClassOf rdf:resource="http://www.semanticweb.org/lenovot480s/ontologies/2024/1/19/untitled-ontology-20#OWLClass_6ad58405_d290_4fc5_a401_c2e4b77343eb"/>
        <rdfs:comment>A strategy that adaptively updates the margin threshold during the learning process.</rdfs:comment>
        <rdfs:label xml:lang="en">AdaptiveThresholdSampling</rdfs:label>
    </owl:Class>
    


    <!-- http://www.semanticweb.org/lenovot480s/ontologies/2024/1/19/untitled-ontology-20#OWLClass_61ad510a_f19d_491b_b3df_d3be4ce6f30a -->

    <owl:Class rdf:about="http://www.semanticweb.org/lenovot480s/ontologies/2024/1/19/untitled-ontology-20#OWLClass_61ad510a_f19d_491b_b3df_d3be4ce6f30a">
        <rdfs:subClassOf rdf:resource="http://www.semanticweb.org/lenovot480s/ontologies/2024/1/19/untitled-ontology-20#OWLClass_f9d76460_e9ef_42a9_8aa2_94b6a52b0421"/>
        <rdfs:comment>Selects instances based on active learning. Properties:- Active learning approach	Values:- Membership querying synthesis, - Stream-based selection</rdfs:comment>
        <rdfs:label xml:lang="en">ActiveLearningBasedSampling</rdfs:label>
    </owl:Class>
    


    <!-- http://www.semanticweb.org/lenovot480s/ontologies/2024/1/19/untitled-ontology-20#OWLClass_638bb7a6_9f56_4ea2_8cb1_4c62c2da900d -->

    <owl:Class rdf:about="http://www.semanticweb.org/lenovot480s/ontologies/2024/1/19/untitled-ontology-20#OWLClass_638bb7a6_9f56_4ea2_8cb1_4c62c2da900d">
        <rdfs:subClassOf rdf:resource="http://www.semanticweb.org/lenovot480s/ontologies/2024/1/19/untitled-ontology-20#OWLClass_5949f4eb_04af_4e5f_a45b_67e5c4d21427"/>
        <rdfs:comment xml:lang="en">Updates the model incrementally as data becomes available.Properties:- Incremental update method. Values- Online gradient descent, - Perceptron update, - Hebbian learning</rdfs:comment>
        <rdfs:label xml:lang="en">IncrementalLearning</rdfs:label>
    </owl:Class>
    


    <!-- http://www.semanticweb.org/lenovot480s/ontologies/2024/1/19/untitled-ontology-20#OWLClass_65d97c3f_0985_4cc3_8fe1_c08ed98db7d4 -->

    <owl:Class rdf:about="http://www.semanticweb.org/lenovot480s/ontologies/2024/1/19/untitled-ontology-20#OWLClass_65d97c3f_0985_4cc3_8fe1_c08ed98db7d4">
        <rdfs:subClassOf rdf:resource="http://www.semanticweb.org/lenovot480s/ontologies/2024/1/19/untitled-ontology-20#OWLClass_c8b11866_3183_47ae_be50_a8e1a8186d37"/>
        <rdfs:comment>A strategy that selects instances with low entropy.</rdfs:comment>
        <rdfs:label xml:lang="en">LowEntropySampling</rdfs:label>
    </owl:Class>
    


    <!-- http://www.semanticweb.org/lenovot480s/ontologies/2024/1/19/untitled-ontology-20#OWLClass_6ad58405_d290_4fc5_a401_c2e4b77343eb -->

    <owl:Class rdf:about="http://www.semanticweb.org/lenovot480s/ontologies/2024/1/19/untitled-ontology-20#OWLClass_6ad58405_d290_4fc5_a401_c2e4b77343eb">
        <rdfs:subClassOf rdf:resource="http://www.semanticweb.org/lenovot480s/ontologies/2024/1/19/untitled-ontology-20#OWLClass_9f328153_8e29_4394_857a_48f04d38d710"/>
        <rdfs:comment>A strategy that selects instances based on a predefined margin threshold.</rdfs:comment>
        <rdfs:label xml:lang="en">MarginThresholdSampling</rdfs:label>
    </owl:Class>
    


    <!-- http://www.semanticweb.org/lenovot480s/ontologies/2024/1/19/untitled-ontology-20#OWLClass_6e05a615_c28f_4a12_bc4e_18eab0ff35a5 -->

    <owl:Class rdf:about="http://www.semanticweb.org/lenovot480s/ontologies/2024/1/19/untitled-ontology-20#OWLClass_6e05a615_c28f_4a12_bc4e_18eab0ff35a5">
        <rdfs:subClassOf rdf:resource="http://www.semanticweb.org/lenovot480s/ontologies/2024/1/19/untitled-ontology-20#OWLClass_f2a74229_b0e1_41b7_b9b9_feec1458e800"/>
        <rdfs:comment xml:lang="en">A strategy that selects instances based on hierarchical clustering. Value: Cluster linkage method (e.g., single, complete)</rdfs:comment>
        <rdfs:label xml:lang="en">HierarchicalSampling</rdfs:label>
    </owl:Class>
    


    <!-- http://www.semanticweb.org/lenovot480s/ontologies/2024/1/19/untitled-ontology-20#OWLClass_70b9ea55_e75c_4759_85cc_cd0014dd7b2f -->

    <owl:Class rdf:about="http://www.semanticweb.org/lenovot480s/ontologies/2024/1/19/untitled-ontology-20#OWLClass_70b9ea55_e75c_4759_85cc_cd0014dd7b2f">
        <rdfs:subClassOf rdf:resource="http://www.semanticweb.org/lenovot480s/ontologies/2024/1/19/untitled-ontology-20#OWLClass_3b0030cc_7a96_45fa_8363_c8c60ab1a0ea"/>
        <rdfs:comment>Active learning scenario with a continuous stream of data.Properties:- Stream speed. Values:- Slow, - Medium, - Fast</rdfs:comment>
        <rdfs:label>StreamBasedScenario</rdfs:label>
    </owl:Class>
    


    <!-- http://www.semanticweb.org/lenovot480s/ontologies/2024/1/19/untitled-ontology-20#OWLClass_7221d6a3_cea1_4532_8672_005b94aaf26a -->

    <owl:Class rdf:about="http://www.semanticweb.org/lenovot480s/ontologies/2024/1/19/untitled-ontology-20#OWLClass_7221d6a3_cea1_4532_8672_005b94aaf26a">
        <rdfs:subClassOf rdf:resource="http://www.semanticweb.org/lenovot480s/ontologies/2024/1/19/untitled-ontology-20#OWLClass_19084a6d_45d5_4ca2_b0e5_1f26c52bcd2f"/>
        <rdfs:comment xml:lang="en">A strategy that selects instances with high variation ratios.</rdfs:comment>
        <rdfs:label xml:lang="en">HighVariationRatioSampling</rdfs:label>
    </owl:Class>
    


    <!-- http://www.semanticweb.org/lenovot480s/ontologies/2024/1/19/untitled-ontology-20#OWLClass_73964c37_b7aa_4290_8c13_5ff4385ef57a -->

    <owl:Class rdf:about="http://www.semanticweb.org/lenovot480s/ontologies/2024/1/19/untitled-ontology-20#OWLClass_73964c37_b7aa_4290_8c13_5ff4385ef57a">
        <rdfs:subClassOf rdf:resource="http://www.semanticweb.org/lenovot480s/ontologies/2024/1/19/untitled-ontology-20#OWLClass_5949f4eb_04af_4e5f_a45b_67e5c4d21427"/>
        <rdfs:comment>Fine-tunes the model on specific task or domain. Property:- Fine-tuning approach.Value:	- Task-specific, - Domain-specific, - Layer-specific</rdfs:comment>
        <rdfs:label xml:lang="en">FineTuning</rdfs:label>
    </owl:Class>
    


    <!-- http://www.semanticweb.org/lenovot480s/ontologies/2024/1/19/untitled-ontology-20#OWLClass_7415d329_9710_4924_a817_8636fe5f2809 -->

    <owl:Class rdf:about="http://www.semanticweb.org/lenovot480s/ontologies/2024/1/19/untitled-ontology-20#OWLClass_7415d329_9710_4924_a817_8636fe5f2809">
        <rdfs:subClassOf rdf:resource="http://www.semanticweb.org/lenovot480s/ontologies/2024/1/19/untitled-ontology-20#OWLClass_f9d76460_e9ef_42a9_8aa2_94b6a52b0421"/>
        <rdfs:comment xml:lang="en">Selects instances based on committee agreement. Properties: Committee size. Values:- Small, - Medium, - Large</rdfs:comment>
        <rdfs:label xml:lang="en">QueryByCommittee</rdfs:label>
    </owl:Class>
    


    <!-- http://www.semanticweb.org/lenovot480s/ontologies/2024/1/19/untitled-ontology-20#OWLClass_76f9b46e_6406_485c_91b9_8fe23f1da1b4 -->

    <owl:Class rdf:about="http://www.semanticweb.org/lenovot480s/ontologies/2024/1/19/untitled-ontology-20#OWLClass_76f9b46e_6406_485c_91b9_8fe23f1da1b4">
        <rdfs:subClassOf rdf:resource="http://www.semanticweb.org/lenovot480s/ontologies/2024/1/19/untitled-ontology-20#OWLClass_19084a6d_45d5_4ca2_b0e5_1f26c52bcd2f"/>
        <rdfs:comment xml:lang="en">A strategy that selects instances with balanced variation ratios.</rdfs:comment>
        <rdfs:label xml:lang="en">BalancedVariationRatioSampling</rdfs:label>
    </owl:Class>
    


    <!-- http://www.semanticweb.org/lenovot480s/ontologies/2024/1/19/untitled-ontology-20#OWLClass_77b2dedc_e0b3_44f5_b46f_ebbfb9aafd93 -->

    <owl:Class rdf:about="http://www.semanticweb.org/lenovot480s/ontologies/2024/1/19/untitled-ontology-20#OWLClass_77b2dedc_e0b3_44f5_b46f_ebbfb9aafd93">
        <rdfs:subClassOf rdf:resource="http://www.semanticweb.org/lenovot480s/ontologies/2024/1/19/untitled-ontology-20#OWLClass_f2a74229_b0e1_41b7_b9b9_feec1458e800"/>
        <rdfs:comment xml:lang="en">A strategy that selects instances based on DBSCAN clustering. Value: Minimum cluster size, epsilon value</rdfs:comment>
        <rdfs:label xml:lang="en">DBSCANSampling</rdfs:label>
    </owl:Class>
    


    <!-- http://www.semanticweb.org/lenovot480s/ontologies/2024/1/19/untitled-ontology-20#OWLClass_78554545_e115_4ae4_9f5f_9b14e0808387 -->

    <owl:Class rdf:about="http://www.semanticweb.org/lenovot480s/ontologies/2024/1/19/untitled-ontology-20#OWLClass_78554545_e115_4ae4_9f5f_9b14e0808387">
        <rdfs:subClassOf rdf:resource="http://www.semanticweb.org/lenovot480s/ontologies/2024/1/19/untitled-ontology-20#OWLClass_da97fd0b_a17c_4ecb_be57_d12afa99ff07"/>
        <rdfs:comment>A strategy that selects instances with margin ranks above a certain threshold. Value:Margin rank threshold value (e.g., 0.8)</rdfs:comment>
        <rdfs:label xml:lang="en">ThresholdedMarginRankingSampling</rdfs:label>
    </owl:Class>
    


    <!-- http://www.semanticweb.org/lenovot480s/ontologies/2024/1/19/untitled-ontology-20#OWLClass_79accebf_1c3a_45e5_bf9c_e4fb7ae53538 -->

    <owl:Class rdf:about="http://www.semanticweb.org/lenovot480s/ontologies/2024/1/19/untitled-ontology-20#OWLClass_79accebf_1c3a_45e5_bf9c_e4fb7ae53538">
        <rdfs:subClassOf rdf:resource="http://www.semanticweb.org/lenovot480s/ontologies/2024/1/19/untitled-ontology-20#OWLClass_1d814d5b_e4fa_40db_bf4b_3d43ee31a2d7"/>
        <rdfs:comment xml:lang="en">A dataset with labeled instances.Properties: &quot;Labeling method, Number of labeled instances, Modality&quot;</rdfs:comment>
        <rdfs:label xml:lang="en">LabeledDataset</rdfs:label>
    </owl:Class>
    


    <!-- http://www.semanticweb.org/lenovot480s/ontologies/2024/1/19/untitled-ontology-20#OWLClass_869fe8b2_903d_4195_9699_c9f12fe26c7f -->

    <owl:Class rdf:about="http://www.semanticweb.org/lenovot480s/ontologies/2024/1/19/untitled-ontology-20#OWLClass_869fe8b2_903d_4195_9699_c9f12fe26c7f">
        <rdfs:subClassOf rdf:resource="http://www.semanticweb.org/lenovot480s/ontologies/2024/1/19/untitled-ontology-20#OWLClass_6ad58405_d290_4fc5_a401_c2e4b77343eb"/>
        <rdfs:comment>A strategy that dynamically adjusts the margin threshold based on data characteristics.</rdfs:comment>
        <rdfs:label xml:lang="en">DynamicThresholdSampling</rdfs:label>
    </owl:Class>
    


    <!-- http://www.semanticweb.org/lenovot480s/ontologies/2024/1/19/untitled-ontology-20#OWLClass_88b2ff0b_e42d_4e0e_99a0_ec37ab4c742f -->

    <owl:Class rdf:about="http://www.semanticweb.org/lenovot480s/ontologies/2024/1/19/untitled-ontology-20#OWLClass_88b2ff0b_e42d_4e0e_99a0_ec37ab4c742f">
        <rdfs:subClassOf rdf:resource="http://www.semanticweb.org/lenovot480s/ontologies/2024/1/19/untitled-ontology-20#OWLClass_b26a3692_a66f_4c78_81f6_fd893eda3095"/>
        <rdfs:comment>A strategy that selects instances to reduce uncertainty in the model.</rdfs:comment>
        <rdfs:label xml:lang="en">UncertaintyReduction</rdfs:label>
    </owl:Class>
    


    <!-- http://www.semanticweb.org/lenovot480s/ontologies/2024/1/19/untitled-ontology-20#OWLClass_8c17eef7_bded_47fe_9121_88360fcce2da -->

    <owl:Class rdf:about="http://www.semanticweb.org/lenovot480s/ontologies/2024/1/19/untitled-ontology-20#OWLClass_8c17eef7_bded_47fe_9121_88360fcce2da">
        <rdfs:subClassOf rdf:resource="http://www.semanticweb.org/lenovot480s/ontologies/2024/1/19/untitled-ontology-20#OWLClass_ddcafd3a_7b94_404c_9c2b_c92ebf4f89e0"/>
        <rdfs:comment xml:lang="en">A strategy that combines active and passive learning approaches.</rdfs:comment>
        <rdfs:label xml:lang="en">ActivePassiveHybrid</rdfs:label>
    </owl:Class>
    


    <!-- http://www.semanticweb.org/lenovot480s/ontologies/2024/1/19/untitled-ontology-20#OWLClass_954bbe2a_1a9d_4a14_919c_dcb51597ef8c -->

    <owl:Class rdf:about="http://www.semanticweb.org/lenovot480s/ontologies/2024/1/19/untitled-ontology-20#OWLClass_954bbe2a_1a9d_4a14_919c_dcb51597ef8c">
        <rdfs:subClassOf rdf:resource="http://www.semanticweb.org/lenovot480s/ontologies/2024/1/19/untitled-ontology-20#OWLClass_3b0030cc_7a96_45fa_8363_c8c60ab1a0ea"/>
        <rdfs:comment>Active learning scenario with resource constraints.Properties:- Budget allocation. Values:- High budget, - Medium budget, - Low budget</rdfs:comment>
        <rdfs:label xml:lang="en">ResourceConstraintScenario</rdfs:label>
    </owl:Class>
    


    <!-- http://www.semanticweb.org/lenovot480s/ontologies/2024/1/19/untitled-ontology-20#OWLClass_97849fb2_d699_48bb_b61f_df0147958e90 -->

    <owl:Class rdf:about="http://www.semanticweb.org/lenovot480s/ontologies/2024/1/19/untitled-ontology-20#OWLClass_97849fb2_d699_48bb_b61f_df0147958e90">
        <rdfs:subClassOf rdf:resource="http://www.semanticweb.org/lenovot480s/ontologies/2024/1/19/untitled-ontology-20#OWLClass_1d814d5b_e4fa_40db_bf4b_3d43ee31a2d7"/>
        <rdfs:comment xml:lang="en">A dataset with a combination of labeled and unlabeled instances.Properties:Labeling ratio, Modality</rdfs:comment>
        <rdfs:label xml:lang="en">SemiSupervisedDataset</rdfs:label>
    </owl:Class>
    


    <!-- http://www.semanticweb.org/lenovot480s/ontologies/2024/1/19/untitled-ontology-20#OWLClass_99779c0f_ac3e_4a63_bafd_98dfcad0db0f -->

    <owl:Class rdf:about="http://www.semanticweb.org/lenovot480s/ontologies/2024/1/19/untitled-ontology-20#OWLClass_99779c0f_ac3e_4a63_bafd_98dfcad0db0f">
        <rdfs:subClassOf rdf:resource="http://www.semanticweb.org/lenovot480s/ontologies/2024/1/19/untitled-ontology-20#OWLClass_3e57c330_a8cc_48c0_afa0_daa39ae53ad8"/>
        <rdfs:label xml:lang="en">ActiveLearningDataset_V.2</rdfs:label>
    </owl:Class>
    


    <!-- http://www.semanticweb.org/lenovot480s/ontologies/2024/1/19/untitled-ontology-20#OWLClass_9d48eb9f_e250_40d7_a2cb_e850829127f2 -->

    <owl:Class rdf:about="http://www.semanticweb.org/lenovot480s/ontologies/2024/1/19/untitled-ontology-20#OWLClass_9d48eb9f_e250_40d7_a2cb_e850829127f2">
        <rdfs:subClassOf rdf:resource="http://www.semanticweb.org/lenovot480s/ontologies/2024/1/19/untitled-ontology-20#OWLClass_1d814d5b_e4fa_40db_bf4b_3d43ee31a2d7"/>
        <rdfs:comment xml:lang="en">A dataset that is continuously updated or streamed.Properties:Streaming method, Modality</rdfs:comment>
        <rdfs:label xml:lang="en">StreamingDataset</rdfs:label>
    </owl:Class>
    


    <!-- http://www.semanticweb.org/lenovot480s/ontologies/2024/1/19/untitled-ontology-20#OWLClass_9dea17b2_2b70_46ea_ac82_8494b9e2b8d9 -->

    <owl:Class rdf:about="http://www.semanticweb.org/lenovot480s/ontologies/2024/1/19/untitled-ontology-20#OWLClass_9dea17b2_2b70_46ea_ac82_8494b9e2b8d9">
        <rdfs:subClassOf rdf:resource="http://www.semanticweb.org/lenovot480s/ontologies/2024/1/19/untitled-ontology-20#OWLClass_48a72743_be39_4bbe_b5d2_9c40286910d1"/>
        <rdfs:comment>A strategy that selects instances to maximize diversity in the training set.</rdfs:comment>
        <rdfs:label xml:lang="en">DiversitySampling</rdfs:label>
    </owl:Class>
    


    <!-- http://www.semanticweb.org/lenovot480s/ontologies/2024/1/19/untitled-ontology-20#OWLClass_9f328153_8e29_4394_857a_48f04d38d710 -->

    <owl:Class rdf:about="http://www.semanticweb.org/lenovot480s/ontologies/2024/1/19/untitled-ontology-20#OWLClass_9f328153_8e29_4394_857a_48f04d38d710">
        <rdfs:subClassOf rdf:resource="http://www.semanticweb.org/lenovot480s/ontologies/2024/1/19/untitled-ontology-20#OWLClass_b476dd4b_0380_4dca_9da6_1bd7e8cd574f"/>
        <rdfs:comment>A strategy that selects instances based on margin uncertainty.</rdfs:comment>
        <rdfs:label xml:lang="en">MarginSampling</rdfs:label>
    </owl:Class>
    


    <!-- http://www.semanticweb.org/lenovot480s/ontologies/2024/1/19/untitled-ontology-20#OWLClass_a08e68ab_9296_4aff_9fe7_366c57f91cb8 -->

    <owl:Class rdf:about="http://www.semanticweb.org/lenovot480s/ontologies/2024/1/19/untitled-ontology-20#OWLClass_a08e68ab_9296_4aff_9fe7_366c57f91cb8">
        <rdfs:subClassOf rdf:resource="http://www.semanticweb.org/lenovot480s/ontologies/2024/1/19/untitled-ontology-20#OWLClass_fef00ae7_b551_4050_80d4_d530b152590f"/>
        <rdfs:comment>Active learning framework combining multiple strategies.Properties:- Component frameworks.Values:- Query-based &amp; Model-based, - Query-based &amp; Transfer learning, - Model-based &amp; Ensemble learning</rdfs:comment>
        <rdfs:label xml:lang="en">HybridFramework</rdfs:label>
    </owl:Class>
    


    <!-- http://www.semanticweb.org/lenovot480s/ontologies/2024/1/19/untitled-ontology-20#OWLClass_a861954a_2366_4a42_9ee6_7e6310841c9e -->

    <owl:Class rdf:about="http://www.semanticweb.org/lenovot480s/ontologies/2024/1/19/untitled-ontology-20#OWLClass_a861954a_2366_4a42_9ee6_7e6310841c9e">
        <rdfs:subClassOf rdf:resource="http://www.semanticweb.org/lenovot480s/ontologies/2024/1/19/untitled-ontology-20#OWLClass_3b0030cc_7a96_45fa_8363_c8c60ab1a0ea"/>
        <rdfs:comment>Active learning scenario focusing on label efficiency.Properties:- Labeling cost.Values:- High cost, - Medium cost, - Low cost</rdfs:comment>
        <rdfs:label xml:lang="en">LabelEfficiencyScenario</rdfs:label>
    </owl:Class>
    


    <!-- http://www.semanticweb.org/lenovot480s/ontologies/2024/1/19/untitled-ontology-20#OWLClass_ae559204_5311_4ca4_9a41_a26f435fb162 -->

    <owl:Class rdf:about="http://www.semanticweb.org/lenovot480s/ontologies/2024/1/19/untitled-ontology-20#OWLClass_ae559204_5311_4ca4_9a41_a26f435fb162">
        <rdfs:subClassOf rdf:resource="http://www.semanticweb.org/lenovot480s/ontologies/2024/1/19/untitled-ontology-20#OWLClass_c13d0274_448e_45df_a089_4f811c399630"/>
        <rdfs:comment xml:lang="en">A strategy that selects representative instances based on prototype selection techniques. Value: Number of prototypes, similarity threshold</rdfs:comment>
        <rdfs:label xml:lang="en">PrototypeSelection</rdfs:label>
    </owl:Class>
    


    <!-- http://www.semanticweb.org/lenovot480s/ontologies/2024/1/19/untitled-ontology-20#OWLClass_b26a3692_a66f_4c78_81f6_fd893eda3095 -->

    <owl:Class rdf:about="http://www.semanticweb.org/lenovot480s/ontologies/2024/1/19/untitled-ontology-20#OWLClass_b26a3692_a66f_4c78_81f6_fd893eda3095">
        <rdfs:subClassOf rdf:resource="http://www.semanticweb.org/lenovot480s/ontologies/2024/1/19/untitled-ontology-20#OWLClass_48a72743_be39_4bbe_b5d2_9c40286910d1"/>
        <rdfs:comment>A strategy that selects instances based on expected changes in the model.</rdfs:comment>
        <rdfs:label xml:lang="en">ExpectedModelChange</rdfs:label>
    </owl:Class>
    


    <!-- http://www.semanticweb.org/lenovot480s/ontologies/2024/1/19/untitled-ontology-20#OWLClass_b476dd4b_0380_4dca_9da6_1bd7e8cd574f -->

    <owl:Class rdf:about="http://www.semanticweb.org/lenovot480s/ontologies/2024/1/19/untitled-ontology-20#OWLClass_b476dd4b_0380_4dca_9da6_1bd7e8cd574f">
        <rdfs:subClassOf rdf:resource="http://www.semanticweb.org/lenovot480s/ontologies/2024/1/19/untitled-ontology-20#OWLClass_48a72743_be39_4bbe_b5d2_9c40286910d1"/>
        <rdfs:comment>A strategy that selects instances based on their uncertainty in prediction.</rdfs:comment>
        <rdfs:label xml:lang="en">UncertaintySampling</rdfs:label>
    </owl:Class>
    


    <!-- http://www.semanticweb.org/lenovot480s/ontologies/2024/1/19/untitled-ontology-20#OWLClass_b5561519_b323_4331_8c29_00ff248fde23 -->

    <owl:Class rdf:about="http://www.semanticweb.org/lenovot480s/ontologies/2024/1/19/untitled-ontology-20#OWLClass_b5561519_b323_4331_8c29_00ff248fde23">
        <rdfs:subClassOf rdf:resource="http://www.semanticweb.org/lenovot480s/ontologies/2024/1/19/untitled-ontology-20#OWLClass_5949f4eb_04af_4e5f_a45b_67e5c4d21427"/>
        <rdfs:comment xml:lang="en">Adjusts the learning rate based on model performance.Properties:- Learning rate adaptation method. Values:- Adagrad, - RMSprop, - Adam</rdfs:comment>
        <rdfs:label xml:lang="en">AdaptiveLearningRate</rdfs:label>
    </owl:Class>
    


    <!-- http://www.semanticweb.org/lenovot480s/ontologies/2024/1/19/untitled-ontology-20#OWLClass_b5b25f53_0cc1_4d4c_a048_5281226d59f9 -->

    <owl:Class rdf:about="http://www.semanticweb.org/lenovot480s/ontologies/2024/1/19/untitled-ontology-20#OWLClass_b5b25f53_0cc1_4d4c_a048_5281226d59f9">
        <rdfs:subClassOf rdf:resource="http://www.semanticweb.org/lenovot480s/ontologies/2024/1/19/untitled-ontology-20#OWLClass_2d55bf6b_29fe_467e_8a00_6d4bab026699"/>
        <rdfs:comment>A strategy that selects instances with a negative margin.</rdfs:comment>
        <rdfs:label xml:lang="en">NegativeMarginSampling</rdfs:label>
    </owl:Class>
    


    <!-- http://www.semanticweb.org/lenovot480s/ontologies/2024/1/19/untitled-ontology-20#OWLClass_b6659e73_efe3_4cfc_a7a6_f5d0ae2b14fe -->

    <owl:Class rdf:about="http://www.semanticweb.org/lenovot480s/ontologies/2024/1/19/untitled-ontology-20#OWLClass_b6659e73_efe3_4cfc_a7a6_f5d0ae2b14fe">
        <rdfs:subClassOf rdf:resource="http://www.semanticweb.org/lenovot480s/ontologies/2024/1/19/untitled-ontology-20#OWLClass_f9d76460_e9ef_42a9_8aa2_94b6a52b0421"/>
        <rdfs:comment>Selects instances randomly. N/A, N/A</rdfs:comment>
        <rdfs:label xml:lang="en">RandomSampling</rdfs:label>
    </owl:Class>
    


    <!-- http://www.semanticweb.org/lenovot480s/ontologies/2024/1/19/untitled-ontology-20#OWLClass_b67da060_5416_4507_b69a_90214af54f68 -->

    <owl:Class rdf:about="http://www.semanticweb.org/lenovot480s/ontologies/2024/1/19/untitled-ontology-20#OWLClass_b67da060_5416_4507_b69a_90214af54f68">
        <rdfs:subClassOf rdf:resource="http://www.semanticweb.org/lenovot480s/ontologies/2024/1/19/untitled-ontology-20#OWLClass_6ad58405_d290_4fc5_a401_c2e4b77343eb"/>
        <rdfs:comment>A strategy that selects instances with a fixed margin threshold. Value: Fixed margin threshold value (e.g., 0.1)</rdfs:comment>
        <rdfs:label xml:lang="en">FixedThresholdSampling</rdfs:label>
    </owl:Class>
    


    <!-- http://www.semanticweb.org/lenovot480s/ontologies/2024/1/19/untitled-ontology-20#OWLClass_b8e3e03e_b55a_4da3_9bcc_af4c663c793a -->

    <owl:Class rdf:about="http://www.semanticweb.org/lenovot480s/ontologies/2024/1/19/untitled-ontology-20#OWLClass_b8e3e03e_b55a_4da3_9bcc_af4c663c793a">
        <rdfs:subClassOf rdf:resource="http://www.semanticweb.org/lenovot480s/ontologies/2024/1/19/untitled-ontology-20#OWLClass_1d814d5b_e4fa_40db_bf4b_3d43ee31a2d7"/>
        <rdfs:comment xml:lang="en">A dataset with unlabeled instances.Properties:Modality</rdfs:comment>
        <rdfs:label xml:lang="en">UnlabeledDataset</rdfs:label>
    </owl:Class>
    


    <!-- http://www.semanticweb.org/lenovot480s/ontologies/2024/1/19/untitled-ontology-20#OWLClass_b9d2b99c_53c7_4cfc_9b25_6f72df8837df -->

    <owl:Class rdf:about="http://www.semanticweb.org/lenovot480s/ontologies/2024/1/19/untitled-ontology-20#OWLClass_b9d2b99c_53c7_4cfc_9b25_6f72df8837df">
        <rdfs:subClassOf rdf:resource="http://www.semanticweb.org/lenovot480s/ontologies/2024/1/19/untitled-ontology-20#OWLClass_5949f4eb_04af_4e5f_a45b_67e5c4d21427"/>
        <rdfs:comment xml:lang="en">Uses model&apos;s predictions to label unlabeled data.Properties:- Confidence threshold Values:- High confidence, - Medium confidence, - Low confidence</rdfs:comment>
        <rdfs:label xml:lang="en">SelfTraining</rdfs:label>
    </owl:Class>
    


    <!-- http://www.semanticweb.org/lenovot480s/ontologies/2024/1/19/untitled-ontology-20#OWLClass_c13d0274_448e_45df_a089_4f811c399630 -->

    <owl:Class rdf:about="http://www.semanticweb.org/lenovot480s/ontologies/2024/1/19/untitled-ontology-20#OWLClass_c13d0274_448e_45df_a089_4f811c399630">
        <rdfs:subClassOf rdf:resource="http://www.semanticweb.org/lenovot480s/ontologies/2024/1/19/untitled-ontology-20#OWLClass_9dea17b2_2b70_46ea_ac82_8494b9e2b8d9"/>
        <rdfs:comment xml:lang="en">A strategy that selects representative instances to maximize diversity.</rdfs:comment>
        <rdfs:label xml:lang="en">RepresentativeSampling</rdfs:label>
    </owl:Class>
    


    <!-- http://www.semanticweb.org/lenovot480s/ontologies/2024/1/19/untitled-ontology-20#OWLClass_c54bb088_7d48_4ea0_868d_8f740315032a -->

    <owl:Class rdf:about="http://www.semanticweb.org/lenovot480s/ontologies/2024/1/19/untitled-ontology-20#OWLClass_c54bb088_7d48_4ea0_868d_8f740315032a">
        <rdfs:subClassOf rdf:resource="http://www.semanticweb.org/lenovot480s/ontologies/2024/1/19/untitled-ontology-20#OWLClass_fef00ae7_b551_4050_80d4_d530b152590f"/>
        <rdfs:comment>Active learning framework adapting to different domains.Properties:- Domain adaptation. Values:- Similar domain adaptation, - Transfer learning, - Meta-learning</rdfs:comment>
        <rdfs:label xml:lang="en">DomainAdaptiveFramework</rdfs:label>
    </owl:Class>
    


    <!-- http://www.semanticweb.org/lenovot480s/ontologies/2024/1/19/untitled-ontology-20#OWLClass_c8b11866_3183_47ae_be50_a8e1a8186d37 -->

    <owl:Class rdf:about="http://www.semanticweb.org/lenovot480s/ontologies/2024/1/19/untitled-ontology-20#OWLClass_c8b11866_3183_47ae_be50_a8e1a8186d37">
        <rdfs:subClassOf rdf:resource="http://www.semanticweb.org/lenovot480s/ontologies/2024/1/19/untitled-ontology-20#OWLClass_b476dd4b_0380_4dca_9da6_1bd7e8cd574f"/>
        <rdfs:comment>A strategy that selects instances based on entropy uncertainty.</rdfs:comment>
        <rdfs:label xml:lang="en">EntropySampling</rdfs:label>
    </owl:Class>
    


    <!-- http://www.semanticweb.org/lenovot480s/ontologies/2024/1/19/untitled-ontology-20#OWLClass_ca099869_170b_4c5d_84bd_7d2463183f9e -->

    <owl:Class rdf:about="http://www.semanticweb.org/lenovot480s/ontologies/2024/1/19/untitled-ontology-20#OWLClass_ca099869_170b_4c5d_84bd_7d2463183f9e">
        <rdfs:subClassOf rdf:resource="http://www.semanticweb.org/lenovot480s/ontologies/2024/1/19/untitled-ontology-20#OWLClass_5949f4eb_04af_4e5f_a45b_67e5c4d21427"/>
        <rdfs:comment xml:lang="en">Retrains the model periodically on new data. Properties:- Retraining frequency. Values:	- Daily, - Weekly, - Monthly</rdfs:comment>
        <rdfs:label xml:lang="en">Retraining</rdfs:label>
    </owl:Class>
    


    <!-- http://www.semanticweb.org/lenovot480s/ontologies/2024/1/19/untitled-ontology-20#OWLClass_ca4abc97_1e1c_4e36_8a8c_104751624977 -->

    <owl:Class rdf:about="http://www.semanticweb.org/lenovot480s/ontologies/2024/1/19/untitled-ontology-20#OWLClass_ca4abc97_1e1c_4e36_8a8c_104751624977">
        <rdfs:subClassOf rdf:resource="http://www.semanticweb.org/lenovot480s/ontologies/2024/1/19/untitled-ontology-20#OWLClass_f2a74229_b0e1_41b7_b9b9_feec1458e800"/>
        <rdfs:comment xml:lang="en">A strategy that selects instances based on K-means clustering. Value:Number of clusters (e.g., K value)</rdfs:comment>
        <rdfs:label xml:lang="en">KMeansSampling</rdfs:label>
    </owl:Class>
    


    <!-- http://www.semanticweb.org/lenovot480s/ontologies/2024/1/19/untitled-ontology-20#OWLClass_cf7afed9_fea8_40d1_9e7b_2e02455d662f -->

    <owl:Class rdf:about="http://www.semanticweb.org/lenovot480s/ontologies/2024/1/19/untitled-ontology-20#OWLClass_cf7afed9_fea8_40d1_9e7b_2e02455d662f">
        <rdfs:subClassOf rdf:resource="http://www.semanticweb.org/lenovot480s/ontologies/2024/1/19/untitled-ontology-20#OWLClass_fef00ae7_b551_4050_80d4_d530b152590f"/>
        <rdfs:comment>Active learning framework based on query strategies.Properties:	- Query strategy	- Uncertainty sampling, - Margin sampling, - Diversity sampling</rdfs:comment>
        <rdfs:label xml:lang="en">QueryBasedFramework</rdfs:label>
    </owl:Class>
    


    <!-- http://www.semanticweb.org/lenovot480s/ontologies/2024/1/19/untitled-ontology-20#OWLClass_da2ff119_8485_4bc8_962a_253ca838a76b -->

    <owl:Class rdf:about="http://www.semanticweb.org/lenovot480s/ontologies/2024/1/19/untitled-ontology-20#OWLClass_da2ff119_8485_4bc8_962a_253ca838a76b">
        <rdfs:subClassOf rdf:resource="http://www.semanticweb.org/lenovot480s/ontologies/2024/1/19/untitled-ontology-20#OWLClass_b26a3692_a66f_4c78_81f6_fd893eda3095"/>
        <rdfs:comment>A strategy that detects changes in the model and selects instances accordingly.</rdfs:comment>
        <rdfs:label xml:lang="en">ModelChangeDetection</rdfs:label>
    </owl:Class>
    


    <!-- http://www.semanticweb.org/lenovot480s/ontologies/2024/1/19/untitled-ontology-20#OWLClass_da7c7c19_a006_477f_b569_6dda0dbcc31d -->

    <owl:Class rdf:about="http://www.semanticweb.org/lenovot480s/ontologies/2024/1/19/untitled-ontology-20#OWLClass_da7c7c19_a006_477f_b569_6dda0dbcc31d">
        <rdfs:subClassOf rdf:resource="http://www.semanticweb.org/lenovot480s/ontologies/2024/1/19/untitled-ontology-20#OWLClass_f2a74229_b0e1_41b7_b9b9_feec1458e800"/>
        <rdfs:comment>A strategy that selects instances based on agglomerative clustering. Value: Linkage criterion (e.g., ward, average)</rdfs:comment>
        <rdfs:label xml:lang="en">AgglomerativeClustering</rdfs:label>
    </owl:Class>
    


    <!-- http://www.semanticweb.org/lenovot480s/ontologies/2024/1/19/untitled-ontology-20#OWLClass_da97fd0b_a17c_4ecb_be57_d12afa99ff07 -->

    <owl:Class rdf:about="http://www.semanticweb.org/lenovot480s/ontologies/2024/1/19/untitled-ontology-20#OWLClass_da97fd0b_a17c_4ecb_be57_d12afa99ff07">
        <rdfs:subClassOf rdf:resource="http://www.semanticweb.org/lenovot480s/ontologies/2024/1/19/untitled-ontology-20#OWLClass_9f328153_8e29_4394_857a_48f04d38d710"/>
        <rdfs:comment>A strategy that selects instances based on ranking by margin uncertainty.</rdfs:comment>
        <rdfs:label xml:lang="en">MarginRankingSampling</rdfs:label>
    </owl:Class>
    


    <!-- http://www.semanticweb.org/lenovot480s/ontologies/2024/1/19/untitled-ontology-20#OWLClass_dbb16834_96c1_4eb9_a90a_8f814a15b95c -->

    <owl:Class rdf:about="http://www.semanticweb.org/lenovot480s/ontologies/2024/1/19/untitled-ontology-20#OWLClass_dbb16834_96c1_4eb9_a90a_8f814a15b95c">
        <rdfs:subClassOf rdf:resource="http://www.semanticweb.org/lenovot480s/ontologies/2024/1/19/untitled-ontology-20#OWLClass_5949f4eb_04af_4e5f_a45b_67e5c4d21427"/>
        <rdfs:comment xml:lang="en">Adapts the model from a related domain or task. Properties:- Source domain. Values:	- Similar domain, - Related task, - Pre-trained model</rdfs:comment>
        <rdfs:label xml:lang="en">TransferLearning</rdfs:label>
    </owl:Class>
    


    <!-- http://www.semanticweb.org/lenovot480s/ontologies/2024/1/19/untitled-ontology-20#OWLClass_dbee48b7_3478_4592_ae24_39a0bbab029f -->

    <owl:Class rdf:about="http://www.semanticweb.org/lenovot480s/ontologies/2024/1/19/untitled-ontology-20#OWLClass_dbee48b7_3478_4592_ae24_39a0bbab029f">
        <rdfs:subClassOf rdf:resource="http://www.semanticweb.org/lenovot480s/ontologies/2024/1/19/untitled-ontology-20#OWLClass_f2a74229_b0e1_41b7_b9b9_feec1458e800"/>
        <rdfs:comment xml:lang="en">A strategy that selects instances based on spectral clustering. Value: Number of clusters, affinity matrix</rdfs:comment>
        <rdfs:label xml:lang="en">SpectralClustering</rdfs:label>
    </owl:Class>
    


    <!-- http://www.semanticweb.org/lenovot480s/ontologies/2024/1/19/untitled-ontology-20#OWLClass_dc75c289_af1b_45ae_8f81_0376a3fd8ec9 -->

    <owl:Class rdf:about="http://www.semanticweb.org/lenovot480s/ontologies/2024/1/19/untitled-ontology-20#OWLClass_dc75c289_af1b_45ae_8f81_0376a3fd8ec9">
        <rdfs:subClassOf rdf:resource="http://www.semanticweb.org/lenovot480s/ontologies/2024/1/19/untitled-ontology-20#OWLClass_b26a3692_a66f_4c78_81f6_fd893eda3095"/>
        <rdfs:comment>A strategy that selects instances to reduce error in the model.</rdfs:comment>
        <rdfs:label xml:lang="en">ErrorReduction</rdfs:label>
    </owl:Class>
    


    <!-- http://www.semanticweb.org/lenovot480s/ontologies/2024/1/19/untitled-ontology-20#OWLClass_dd6e9950_59ef_4b16_a4bc_14abd173f2d6 -->

    <owl:Class rdf:about="http://www.semanticweb.org/lenovot480s/ontologies/2024/1/19/untitled-ontology-20#OWLClass_dd6e9950_59ef_4b16_a4bc_14abd173f2d6">
        <rdfs:subClassOf rdf:resource="http://www.semanticweb.org/lenovot480s/ontologies/2024/1/19/untitled-ontology-20#OWLClass_ddcafd3a_7b94_404c_9c2b_c92ebf4f89e0"/>
        <rdfs:comment xml:lang="en">A strategy that combines multiple active learning models or classifiers. Value: Number of models, aggregation method</rdfs:comment>
        <rdfs:label xml:lang="en">CommitteeBasedHybrid</rdfs:label>
    </owl:Class>
    


    <!-- http://www.semanticweb.org/lenovot480s/ontologies/2024/1/19/untitled-ontology-20#OWLClass_ddcafd3a_7b94_404c_9c2b_c92ebf4f89e0 -->

    <owl:Class rdf:about="http://www.semanticweb.org/lenovot480s/ontologies/2024/1/19/untitled-ontology-20#OWLClass_ddcafd3a_7b94_404c_9c2b_c92ebf4f89e0">
        <rdfs:subClassOf rdf:resource="http://www.semanticweb.org/lenovot480s/ontologies/2024/1/19/untitled-ontology-20#OWLClass_48a72743_be39_4bbe_b5d2_9c40286910d1"/>
        <rdfs:comment>A strategy that combines multiple query strategies for improved performance.</rdfs:comment>
        <rdfs:label xml:lang="en">HybridStrategy</rdfs:label>
    </owl:Class>
    


    <!-- http://www.semanticweb.org/lenovot480s/ontologies/2024/1/19/untitled-ontology-20#OWLClass_ded6530d_092b_4d4f_94a3_a965c66818f4 -->

    <owl:Class rdf:about="http://www.semanticweb.org/lenovot480s/ontologies/2024/1/19/untitled-ontology-20#OWLClass_ded6530d_092b_4d4f_94a3_a965c66818f4">
        <rdfs:subClassOf rdf:resource="http://www.semanticweb.org/lenovot480s/ontologies/2024/1/19/untitled-ontology-20#OWLClass_c13d0274_448e_45df_a089_4f811c399630"/>
        <rdfs:comment xml:lang="en">A strategy that selects representative instances with balanced class distribution. Value: Number of instances per class</rdfs:comment>
        <rdfs:label xml:lang="en">BalancedSampling</rdfs:label>
    </owl:Class>
    


    <!-- http://www.semanticweb.org/lenovot480s/ontologies/2024/1/19/untitled-ontology-20#OWLClass_e3587b1a_351a_40af_a4b0_2448b169856f -->

    <owl:Class rdf:about="http://www.semanticweb.org/lenovot480s/ontologies/2024/1/19/untitled-ontology-20#OWLClass_e3587b1a_351a_40af_a4b0_2448b169856f">
        <rdfs:subClassOf rdf:resource="http://www.semanticweb.org/lenovot480s/ontologies/2024/1/19/untitled-ontology-20#OWLClass_fef00ae7_b551_4050_80d4_d530b152590f"/>
        <rdfs:comment>Active learning framework adapting to specific scenarios.Properties:- Scenario adaptation. Values- Pool-based scenario, - Stream-based scenario, - Real-world scenario</rdfs:comment>
        <rdfs:label xml:lang="en">ScenarioAdaptiveFramework</rdfs:label>
    </owl:Class>
    


    <!-- http://www.semanticweb.org/lenovot480s/ontologies/2024/1/19/untitled-ontology-20#OWLClass_e4814474_c89e_40af_9d8f_13a9f3cb5bc5 -->

    <owl:Class rdf:about="http://www.semanticweb.org/lenovot480s/ontologies/2024/1/19/untitled-ontology-20#OWLClass_e4814474_c89e_40af_9d8f_13a9f3cb5bc5">
        <rdfs:subClassOf rdf:resource="http://www.semanticweb.org/lenovot480s/ontologies/2024/1/19/untitled-ontology-20#OWLClass_19084a6d_45d5_4ca2_b0e5_1f26c52bcd2f"/>
        <rdfs:comment xml:lang="en">A strategy that selects instances with low variation ratios.</rdfs:comment>
        <rdfs:label xml:lang="en">LowVariationRatioSampling</rdfs:label>
    </owl:Class>
    


    <!-- http://www.semanticweb.org/lenovot480s/ontologies/2024/1/19/untitled-ontology-20#OWLClass_e5f4ef9b_d83d_4614_88fc_c53ebc478529 -->

    <owl:Class rdf:about="http://www.semanticweb.org/lenovot480s/ontologies/2024/1/19/untitled-ontology-20#OWLClass_e5f4ef9b_d83d_4614_88fc_c53ebc478529">
        <rdfs:subClassOf rdf:resource="http://www.semanticweb.org/lenovot480s/ontologies/2024/1/19/untitled-ontology-20#OWLClass_5949f4eb_04af_4e5f_a45b_67e5c4d21427"/>
        <rdfs:comment xml:lang="en">Learns to update the model based on past performance.Properties:- Meta-learner type. Values:- Gradient-based, - Memory-based, - Model-based</rdfs:comment>
        <rdfs:label xml:lang="en">MetaLearning</rdfs:label>
    </owl:Class>
    


    <!-- http://www.semanticweb.org/lenovot480s/ontologies/2024/1/19/untitled-ontology-20#OWLClass_e7e26fef_12ca_4b3f_b7fa_ab55335172f7 -->

    <owl:Class rdf:about="http://www.semanticweb.org/lenovot480s/ontologies/2024/1/19/untitled-ontology-20#OWLClass_e7e26fef_12ca_4b3f_b7fa_ab55335172f7">
        <rdfs:subClassOf rdf:resource="http://www.semanticweb.org/lenovot480s/ontologies/2024/1/19/untitled-ontology-20#OWLClass_ddcafd3a_7b94_404c_9c2b_c92ebf4f89e0"/>
        <rdfs:comment xml:lang="en">A strategy that combines diversity and uncertainty sampling approaches.</rdfs:comment>
        <rdfs:label xml:lang="en">DiversityUncertaintyHybrid</rdfs:label>
    </owl:Class>
    


    <!-- http://www.semanticweb.org/lenovot480s/ontologies/2024/1/19/untitled-ontology-20#OWLClass_ed05a0bb_9c01_4606_8670_c90c1581ff03 -->

    <owl:Class rdf:about="http://www.semanticweb.org/lenovot480s/ontologies/2024/1/19/untitled-ontology-20#OWLClass_ed05a0bb_9c01_4606_8670_c90c1581ff03">
        <rdfs:subClassOf rdf:resource="http://www.semanticweb.org/lenovot480s/ontologies/2024/1/19/untitled-ontology-20#OWLClass_f9d76460_e9ef_42a9_8aa2_94b6a52b0421"/>
        <rdfs:comment xml:lang="en">Selects diverse instances to cover data space. Properties:- Diversity measure. Values: - Cluster-based, - Density-based, - Representative-based</rdfs:comment>
        <rdfs:label xml:lang="en">DiversitySampling</rdfs:label>
    </owl:Class>
    


    <!-- http://www.semanticweb.org/lenovot480s/ontologies/2024/1/19/untitled-ontology-20#OWLClass_f24cbbac_1dfe_48d8_a8be_b528858524c2 -->

    <owl:Class rdf:about="http://www.semanticweb.org/lenovot480s/ontologies/2024/1/19/untitled-ontology-20#OWLClass_f24cbbac_1dfe_48d8_a8be_b528858524c2">
        <rdfs:subClassOf rdf:resource="http://www.semanticweb.org/lenovot480s/ontologies/2024/1/19/untitled-ontology-20#OWLClass_3b0030cc_7a96_45fa_8363_c8c60ab1a0ea"/>
        <rdfs:comment>Active learning scenario with a fixed pool of unlabeled instances.	Properties:- Pool size. Values:- Small, - Medium, - Large</rdfs:comment>
        <rdfs:label xml:lang="en">PoolBasedScenario</rdfs:label>
    </owl:Class>
    


    <!-- http://www.semanticweb.org/lenovot480s/ontologies/2024/1/19/untitled-ontology-20#OWLClass_f2a74229_b0e1_41b7_b9b9_feec1458e800 -->

    <owl:Class rdf:about="http://www.semanticweb.org/lenovot480s/ontologies/2024/1/19/untitled-ontology-20#OWLClass_f2a74229_b0e1_41b7_b9b9_feec1458e800">
        <rdfs:subClassOf rdf:resource="http://www.semanticweb.org/lenovot480s/ontologies/2024/1/19/untitled-ontology-20#OWLClass_9dea17b2_2b70_46ea_ac82_8494b9e2b8d9"/>
        <rdfs:comment>A strategy that selects instances from diverse clusters.</rdfs:comment>
        <rdfs:label xml:lang="en">ClusterSampling</rdfs:label>
    </owl:Class>
    


    <!-- http://www.semanticweb.org/lenovot480s/ontologies/2024/1/19/untitled-ontology-20#OWLClass_f44e800e_eb5e_461d_8950_086c424f63ee -->

    <owl:Class rdf:about="http://www.semanticweb.org/lenovot480s/ontologies/2024/1/19/untitled-ontology-20#OWLClass_f44e800e_eb5e_461d_8950_086c424f63ee">
        <rdfs:subClassOf rdf:resource="http://www.semanticweb.org/lenovot480s/ontologies/2024/1/19/untitled-ontology-20#OWLClass_2d55bf6b_29fe_467e_8a00_6d4bab026699"/>
        <rdfs:comment>A strategy that selects instances with a weighted margin based on importance.
Value:Weighting factors for instances</rdfs:comment>
        <rdfs:label xml:lang="en">WeightedMarginSampling</rdfs:label>
    </owl:Class>
    


    <!-- http://www.semanticweb.org/lenovot480s/ontologies/2024/1/19/untitled-ontology-20#OWLClass_f6d14a02_7183_4cf5_8cd7_b493336d571a -->

    <owl:Class rdf:about="http://www.semanticweb.org/lenovot480s/ontologies/2024/1/19/untitled-ontology-20#OWLClass_f6d14a02_7183_4cf5_8cd7_b493336d571a">
        <rdfs:subClassOf rdf:resource="http://www.semanticweb.org/lenovot480s/ontologies/2024/1/19/untitled-ontology-20#OWLClass_f9d76460_e9ef_42a9_8aa2_94b6a52b0421"/>
        <rdfs:comment xml:lang="en">Selects instances with uncertain predictions. Properties:Confidence measure. Values: - Least confident, - Most confident, - Entropy, - Least margin</rdfs:comment>
        <rdfs:label xml:lang="en">UncertaintySampling</rdfs:label>
    </owl:Class>
    


    <!-- http://www.semanticweb.org/lenovot480s/ontologies/2024/1/19/untitled-ontology-20#OWLClass_f7b4bbe4_aaaf_4fcc_a8e5_9e1dc23fd73b -->

    <owl:Class rdf:about="http://www.semanticweb.org/lenovot480s/ontologies/2024/1/19/untitled-ontology-20#OWLClass_f7b4bbe4_aaaf_4fcc_a8e5_9e1dc23fd73b">
        <rdfs:subClassOf rdf:resource="http://www.semanticweb.org/lenovot480s/ontologies/2024/1/19/untitled-ontology-20#OWLClass_c13d0274_448e_45df_a089_4f811c399630"/>
        <rdfs:comment xml:lang="en">A strategy that randomly selects representative instances. Value: Number of instances to select</rdfs:comment>
        <rdfs:label xml:lang="en">RandomSampling</rdfs:label>
    </owl:Class>
    


    <!-- http://www.semanticweb.org/lenovot480s/ontologies/2024/1/19/untitled-ontology-20#OWLClass_f9d76460_e9ef_42a9_8aa2_94b6a52b0421 -->

    <owl:Class rdf:about="http://www.semanticweb.org/lenovot480s/ontologies/2024/1/19/untitled-ontology-20#OWLClass_f9d76460_e9ef_42a9_8aa2_94b6a52b0421">
        <rdfs:subClassOf rdf:resource="http://www.semanticweb.org/lenovot480s/ontologies/2024/1/19/untitled-ontology-20#OWLClass_3e57c330_a8cc_48c0_afa0_daa39ae53ad8"/>
        <rdfs:label xml:lang="en">InstanceSelectionStrategy</rdfs:label>
    </owl:Class>
    


    <!-- http://www.semanticweb.org/lenovot480s/ontologies/2024/1/19/untitled-ontology-20#OWLClass_fef00ae7_b551_4050_80d4_d530b152590f -->

    <owl:Class rdf:about="http://www.semanticweb.org/lenovot480s/ontologies/2024/1/19/untitled-ontology-20#OWLClass_fef00ae7_b551_4050_80d4_d530b152590f">
        <rdfs:subClassOf rdf:resource="http://www.semanticweb.org/lenovot480s/ontologies/2024/1/19/untitled-ontology-20#OWLClass_3e57c330_a8cc_48c0_afa0_daa39ae53ad8"/>
        <rdfs:label xml:lang="en">ActiveLearningFramework</rdfs:label>
    </owl:Class>
    


    <!-- http://www.semanticweb.org/lenovot480s/ontologies/2024/1/19/untitled-ontology-20#OWLClass_ff9fc0da_a3d2_4bac_92fb_1f0906a7e5d4 -->

    <owl:Class rdf:about="http://www.semanticweb.org/lenovot480s/ontologies/2024/1/19/untitled-ontology-20#OWLClass_ff9fc0da_a3d2_4bac_92fb_1f0906a7e5d4">
        <rdfs:subClassOf rdf:resource="http://www.semanticweb.org/lenovot480s/ontologies/2024/1/19/untitled-ontology-20#OWLClass_f9d76460_e9ef_42a9_8aa2_94b6a52b0421"/>
        <rdfs:comment xml:lang="en">Selects instances close to decision boundary. Properties:Margin threshold. Values:- High margin, - Medium margin, - Low margin</rdfs:comment>
        <rdfs:label xml:lang="en">MarginSampling</rdfs:label>
    </owl:Class>
    


    <!-- http://www.semanticweb.org/lenovot480s/ontologies/2024/1/19/untitled-ontology-20#OWLClass_ffdf6a31_fda5_43c2_a011_9de94599f300 -->

    <owl:Class rdf:about="http://www.semanticweb.org/lenovot480s/ontologies/2024/1/19/untitled-ontology-20#OWLClass_ffdf6a31_fda5_43c2_a011_9de94599f300">
        <rdfs:subClassOf rdf:resource="http://www.semanticweb.org/lenovot480s/ontologies/2024/1/19/untitled-ontology-20#OWLClass_c8b11866_3183_47ae_be50_a8e1a8186d37"/>
        <rdfs:comment>A strategy that selects instances with balanced entropy distribution.</rdfs:comment>
        <rdfs:label xml:lang="en">BalancedEntropySampling</rdfs:label>
    </owl:Class>
</rdf:RDF>



<!-- Generated by the OWL API (version 4.5.26.2023-07-17T20:34:13Z) https://github.com/owlcs/owlapi -->

